delay-steps in ZR

Montanari_Weak_Relations.thy
@@ -17,7 +17,7 @@ where
     (\<exists> q'. (q \<Rightarrow>$ A q') \<and> R q' p')\<close>
 
 definition ZR :: "(('s \<Rightarrow> ('s set) \<Rightarrow> bool)) \<Rightarrow> ('s \<Rightarrow> ('s set) \<Rightarrow> bool)" where 
-\<open>ZR R p' Q' \<equiv> \<exists>p Q A. R p Q \<and> p \<Rightarrow>$A p' \<and> (\<forall>a \<in> set A. a \<noteq> \<tau>) \<and> Q' = (succs_seq_rec (rev A) Q)\<close>
+\<open>ZR R p' Q' \<equiv> \<exists>p Q A. R p Q \<and> p \<Rightarrow>$A p' \<and> (\<forall>a \<in> set A. a \<noteq> \<tau>) \<and> Q' = (dsuccs_seq_rec (rev A) Q)\<close>
 
 definition set_type :: "('s \<Rightarrow> 's \<Rightarrow> bool) \<Rightarrow> ('s \<Rightarrow> ('s set) \<Rightarrow> bool)" where 
 \<open>set_type R p Q \<equiv> \<exists>q. R p q \<and> Q = {q}\<close>
@@ -26,7 +26,7 @@ lemma R_is_in_ZR :
   assumes \<open>R p Q\<close>
   shows \<open>ZR R p Q\<close>
 proof -
-  have Q_cond: \<open>Q = succs_seq_rec (rev []) Q\<close>  by simp 
+  have Q_cond: \<open>Q = dsuccs_seq_rec (rev []) Q\<close>  by simp 
   have p_cond: \<open>p \<Rightarrow>$[] p\<close> using steps.simps weak_step_seq.simps(1) by blast 
   thus \<open>ZR R p Q\<close> using Q_cond ZR_def \<open>R p Q\<close>
     by (metis bex_empty empty_set tau_tau)
@@ -37,11 +37,11 @@ lemma ZR_C_guarantees_tau_succ :
     \<open>contrasim C\<close>
     \<open>ZR (set_type C) p Q\<close>
     \<open>p \<Rightarrow>^\<tau> p'\<close>
-  shows \<open>\<exists>q'. q' \<in> (succs \<tau> Q) \<and> ZR (set_type C) q' {p'}\<close>
+  shows \<open>\<exists>q'. q' \<in> (hsuccs \<tau> Q) \<and> ZR (set_type C) q' {p'}\<close>
 proof -
   obtain p0 Q0 A q0
       where \<open>(set_type C) p0 Q0\<close> \<open>p0 \<Rightarrow>$A p\<close> \<open>\<forall>a \<in> set A. a \<noteq> \<tau>\<close> \<open>Q0 = {q0}\<close> 
-        and Q_def: \<open>Q = (succs_seq_rec (rev A) Q0)\<close> 
+        and Q_def: \<open>Q = (dsuccs_seq_rec (rev A) Q0)\<close> 
       using ZR_def assms set_type_def by metis
   hence \<open>C p0 q0\<close> using set_type_def by auto 
   have \<open>p0 \<Rightarrow>$(A@[\<tau>]) p'\<close> using \<open>p0 \<Rightarrow>$A p\<close>  \<open>p \<Rightarrow>^\<tau>  p'\<close> rev_seq_step_concat by auto
@@ -51,23 +51,21 @@ proof -
     using assms contrasim_def[of \<open>C\<close>] \<open>C p0 q0\<close> \<open>\<forall>a \<in> set A. a \<noteq> \<tau>\<close> by blast
   hence \<open>(set_type C) q' {p'}\<close> using set_type_def by auto
   hence inZR: \<open>ZR (set_type C) q' {p'}\<close> using R_is_in_ZR  by auto
-  have \<open>q' \<in> succs \<tau> Q\<close>
+  have \<open>q' \<in> hsuccs \<tau> Q\<close>
   proof (cases \<open>A = []\<close>)
     case True
     hence \<open>q0 \<Rightarrow>^\<tau> q'\<close> using \<open>q0 \<Rightarrow>$A q'\<close> by auto
-    hence \<open>q' \<in> succs \<tau> {q0}\<close> using succs_def by simp
-    hence \<open>q' \<in> succs \<tau> Q0\<close>  using \<open>Q0 = {q0}\<close>  by simp       
-    thus \<open>q' \<in> succs \<tau> Q\<close>  using Q_def by (simp add: True) 
+    hence \<open>q' \<in> hsuccs \<tau> {q0}\<close> using hsuccs_def by simp
+    hence \<open>q' \<in> hsuccs \<tau> Q0\<close>  using \<open>Q0 = {q0}\<close>  by simp       
+    thus \<open>q' \<in> hsuccs \<tau> Q\<close>  using Q_def by (simp add: True) 
   next
     case False
-    hence \<open>q' \<in> succs_seq_rec (rev A) Q0\<close> 
+    hence \<open>q' \<in> hsuccs \<tau> (dsuccs_seq_rec (rev A) Q0)\<close> 
       using \<open>Q0 = {q0}\<close> \<open>q0 \<Rightarrow>$ A q'\<close>
       by (simp add: word_reachable_implies_in_s) 
-    hence \<open>q' \<in> Q\<close> using Q_def by auto
-    hence \<open>\<exists>q \<in> Q. q \<Rightarrow>^\<tau> q'\<close> using \<open>q' \<in> Q\<close> steps.refl by auto
-    thus \<open>q' \<in> succs \<tau> Q\<close>using succs_def by simp
+    thus \<open>q' \<in> hsuccs \<tau> Q\<close> using Q_def by simp 
   qed
-  thus \<open>\<exists>q'. q' \<in> succs \<tau> Q \<and> ZR (set_type C) q' {p'}\<close> using inZR by auto
+  thus \<open>\<exists>q'. q' \<in> hsuccs \<tau> Q \<and> ZR (set_type C) q' {p'}\<close> using inZR by auto
 qed
 
 lemma ZR_C_guarantees_action_succ :
@@ -76,10 +74,11 @@ lemma ZR_C_guarantees_action_succ :
     \<open>ZR (set_type C) p Q\<close>
     \<open>p \<Rightarrow>a p'\<close>
     \<open>a \<noteq> \<tau>\<close>
-  shows \<open>succs a Q \<noteq> {}  \<and> ZR (set_type C) p' (succs a Q)\<close>
+  shows \<open>dsuccs a Q \<noteq> {}  \<and> ZR (set_type C) p' (dsuccs a Q)\<close>
 proof -
   obtain p0 Q0 A q0
-    where \<open>(set_type C) p0 Q0\<close> \<open>p0 \<Rightarrow>$A p\<close> \<open>Q0 = {q0}\<close> \<open>\<forall>a \<in> set A. a \<noteq> \<tau> \<close> and Q_def: \<open>Q = (succs_seq_rec (rev A) Q0)\<close> 
+    where \<open>(set_type C) p0 Q0\<close> \<open>p0 \<Rightarrow>$A p\<close> \<open>Q0 = {q0}\<close> \<open>\<forall>a \<in> set A. a \<noteq> \<tau> \<close> 
+      and Q_def: \<open>Q = (dsuccs_seq_rec (rev A) Q0)\<close> 
     using ZR_def assms set_type_def by metis
   then obtain CS where CS_def: \<open>contrasim CS \<and> CS p0 q0\<close> 
     using assms set_type_def by (metis singleton_inject) 
@@ -91,17 +90,17 @@ proof -
   then obtain q' where \<open>q0 \<Rightarrow>$(A@[a]) q' \<and> CS q' p'\<close> 
     using CS_def contrasim_def[of \<open>CS\<close>] notau
     by fastforce
-  hence in_succs: \<open>q' \<in> (succs_seq_rec (rev (A@[a])) {q0})\<close> 
+  hence \<open>q' \<in> hsuccs \<tau> (dsuccs_seq_rec (rev (A@[a])) {q0})\<close> 
     using word_reachable_implies_in_s by blast
-  hence \<open>q' \<in> (succs_seq_rec (a#(rev A)) {q0})\<close>
-    by (metis rev_eq_Cons_iff rev_rev_ident)
-  hence \<open>q' \<in> succs a (succs_seq_rec (rev A) {q0})\<close> by auto
-  hence notempty: \<open>q' \<in> succs a Q\<close> using Q_def \<open>Q0 = {q0}\<close>  by auto
-  have \<open>ZR (set_type C) p' (succs a Q)\<close> 
-    using in_succs word ZR_def[of \<open>(set_type C)\<close>] \<open>(set_type C) p0 Q0\<close> 
-      \<open>Q0 = {q0}\<close> Q_def simp_succs_seq_rev notau
-    by meson
-  with notempty show \<open>succs a Q \<noteq> {} \<and> ZR (set_type C) p' (succs a Q)\<close> by auto
+  then obtain q1 where in_dsuccs: \<open>q1 \<in> dsuccs_seq_rec (rev (A@[a])) {q0}\<close> \<open>q1 \<Rightarrow>^\<tau> q'\<close>
+    using hsuccs_def[of _ \<open>dsuccs_seq_rec (rev (A@[a])) {q0}\<close>] by auto
+  hence \<open>q1 \<in> dsuccs_seq_rec (a#(rev A)) {q0}\<close> by auto
+  hence \<open>q1 \<in> dsuccs a (dsuccs_seq_rec (rev A) {q0})\<close>  by auto
+  hence notempty: \<open>q1 \<in> dsuccs a Q\<close> using Q_def \<open>Q0 = {q0}\<close> by auto
+  have \<open>ZR (set_type C) p' (dsuccs a Q)\<close> 
+    using in_dsuccs word ZR_def[of \<open>(set_type C)\<close>] \<open>(set_type C) p0 Q0\<close> 
+      \<open>Q0 = {q0}\<close> Q_def notau simp_dsuccs_seq_rev by meson
+  with notempty show ?thesis by auto
 qed
 
 end
